acquireCapacity

concurrency/disciplined/Impl.i.dfy
@@ -100,161 +100,156 @@ module Impl refines VerificationObligation {
     v := Variables.Variables(row_mutexes, allocator);
   }
 
-  // predicate method shouldHashGoBefore(search_h: uint32, slot_h: uint32, slot_idx: uint32) 
-  //   ensures shouldHashGoBefore(search_h, slot_h, slot_idx) == ShouldHashGoBefore(search_h as int, slot_h as int, slot_idx as int)
-  // {
-  //   || search_h < slot_h <= slot_idx // normal case
-  //   || slot_h <= slot_idx < search_h // search_h wraps around the end of array
-  //   || slot_idx < search_h < slot_h// search_h, slot_h wrap around the end of array
-  // }
+  predicate method shouldHashGoBefore(search_h: uint32, slot_h: uint32, slot_idx: uint32) 
+    ensures shouldHashGoBefore(search_h, slot_h, slot_idx) == ShouldHashGoBefore(search_h as int, slot_h as int, slot_idx as int)
+  {
+    || search_h < slot_h <= slot_idx // normal case
+    || slot_h <= slot_idx < search_h // search_h wraps around the end of array
+    || slot_idx < search_h < slot_h// search_h, slot_h wrap around the end of array
+  }
 
-  // function method getNextIndex(slot_idx: uint32) : uint32
-  //   requires slot_idx < FixedSizeImpl()
-  // {
-  //   if slot_idx == FixedSizeImpl() - 1 then 0 else slot_idx + 1
-  // }
+  function method getNextIndex(slot_idx: uint32) : uint32
+    requires slot_idx < FixedSizeImpl()
+  {
+    if slot_idx == FixedSizeImpl() - 1 then 0 else slot_idx + 1
+  }
 
-  // function DistanceToSlot(src: uint32, dst: uint32) : nat
-  //   requires src < FixedSizeImpl()
-  //   requires dst < FixedSizeImpl()
-  // {
-  //   if src >= dst
-  //     then (dst as int - src as int + FixedSize() as int)
-  //     else (dst as int - src as int)
-  // }
+  function DistanceToSlot(src: uint32, dst: uint32) : nat
+    requires src < FixedSizeImpl()
+    requires dst < FixedSizeImpl()
+  {
+    if src >= dst
+      then (dst as int - src as int + FixedSize() as int)
+      else (dst as int - src as int)
+  }
 
-  // method doQuery(v: Variables, input: Ifc.Input, rid: int, glinear in_sv: SSM.Variables)
-  // returns (output: Ifc.Output, glinear out_sv: SSM.Variables)
-  //   decreases *
-  //   requires Inv(v)
-  //   requires input.QueryInput?
-  //   requires isInputResource(in_sv, rid, input)
-  //   ensures out_sv == SSM.output_stub(rid, output)
-  // {
-  //   var query_ticket := Ticket(rid, input);
-  //   var key := input.key;
-  //   var hash_idx := hash(key);
-  //   var slot_idx := hash_idx;
+  method doQuery(v: Variables, input: Ifc.Input, rid: int, glinear in_sv: SSM.Variables)
+  returns (output: Ifc.Output, glinear out_sv: SSM.Variables)
+    decreases *
+    requires Inv(v)
+    requires input.QueryInput?
+    requires isInputResource(in_sv, rid, input)
+    ensures out_sv == SSM.output_stub(rid, output)
+  {
+    var query_ticket := Ticket(rid, input);
+    var key := input.key;
+    var hash_idx := hash(key);
+    var slot_idx := hash_idx;
 
-  //   linear var row; glinear var handle;
-  //   row, handle := v.row_mutexes[slot_idx].acquire();
-  //   linear var Row(entry, row_r) := row;
-  //   glinear var r := SSM.join(in_sv, row_r);
+    linear var row; glinear var handle;
+    row, handle := v.row_mutexes[slot_idx].acquire();
+    linear var Row(entry, row_r) := row;
+    glinear var r := SSM.join(in_sv, row_r);
 
-  //   ghost var r' := oneRowResource(hash_idx as nat, Info(entry, Querying(rid, key)), 0);
-  //   assert ProcessQueryTicket(r, r', query_ticket);
+    ghost var r' := oneRowResource(hash_idx as nat, Info(entry, Querying(rid, key)), 0);
+    assert ProcessQueryTicket(r, r', query_ticket);
 
-  //   var step := ProcessQueryTicketStep(query_ticket);
-  //   r := easy_transform_step(r, r', step);
+    var step := ProcessQueryTicketStep(query_ticket);
+    r := easy_transform_step(r, r', step);
 
-  //   while true 
-  //     invariant Inv(v);
-  //     invariant 0 <= slot_idx < FixedSizeImpl();
-  //     invariant r == oneRowResource(slot_idx as nat, Info(entry, Querying(rid, key)), 0);
-  //     invariant handle.m == v.row_mutexes[slot_idx];
-  //     decreases *
-  //   {
-  //     var slot_idx' := getNextIndex(slot_idx);
+    while true 
+      invariant Inv(v);
+      invariant 0 <= slot_idx < FixedSizeImpl();
+      invariant r == oneRowResource(slot_idx as nat, Info(entry, Querying(rid, key)), 0);
+      invariant handle.m == v.row_mutexes[slot_idx];
+      decreases *
+    {
+      var slot_idx' := getNextIndex(slot_idx);
 
-  //     match entry {
-  //       case Empty => {
-  //         output := MapIfc.QueryOutput(NotFound);
-  //         step := QueryNotFoundStep(slot_idx as nat);
-  //       }
-  //       case Full(KV(entry_key, value)) => {
-  //         if entry_key == key {
-  //           step := QueryDoneStep(slot_idx as nat);
-  //           output := MapIfc.QueryOutput(Found(value));
-  //         } else {
-  //           var should_go_before := shouldHashGoBefore(hash_idx, hash(entry_key), slot_idx);
+      match entry {
+        case Empty => {
+          output := MapIfc.QueryOutput(NotFound);
+          step := QueryNotFoundStep(slot_idx as nat);
+        }
+        case Full(KV(entry_key, value)) => {
+          if entry_key == key {
+            step := QueryDoneStep(slot_idx as nat);
+            output := MapIfc.QueryOutput(Found(value));
+          } else {
+            var should_go_before := shouldHashGoBefore(hash_idx, hash(entry_key), slot_idx);
 
-  //           if !should_go_before {
-  //             step := QuerySkipStep(slot_idx as nat);
-  //           } else {
-  //             output := MapIfc.QueryOutput(NotFound);
-  //             step := QueryNotFoundStep(slot_idx as nat);
-  //           }
-  //         }
-  //       }
-  //     }
+            if !should_go_before {
+              step := QuerySkipStep(slot_idx as nat);
+            } else {
+              output := MapIfc.QueryOutput(NotFound);
+              step := QueryNotFoundStep(slot_idx as nat);
+            }
+          }
+        }
+      }
 
-  //     if !step.QuerySkipStep? {
-  //       // this test is required for termination, but is not enforced by verification
-  //       // because we are using decreases *
-  //       break;
-  //     }
+      if !step.QuerySkipStep? {
+        // this test is required for termination, but is not enforced by verification
+        // because we are using decreases *
+        break;
+      }
 
-  //     // if slot_idx' == hash_idx {
-  //     //   QueryUnreachableState(r, slot_idx as nat);
-  //     //   break;
-  //     // }
+      linear var next_row; glinear var next_handle;
+      next_row, next_handle := v.row_mutexes[slot_idx'].acquire();
+      linear var Row(next_entry, next_row_r) := next_row;
+      r := SSM.join(r, next_row_r);
 
-  //     linear var next_row; glinear var next_handle;
-  //     next_row, next_handle := v.row_mutexes[slot_idx'].acquire();
-  //     linear var Row(next_entry, next_row_r) := next_row;
-  //     r := SSM.join(r, next_row_r);
+      r' := twoRowsResource(slot_idx as nat, Info(entry, Free), slot_idx' as nat, Info(next_entry, Querying(rid, key)), 0);
+      r := easy_transform_step(r, r', step);
 
-  //     r' := twoRowsResource(slot_idx as nat, Info(entry, Free), slot_idx' as nat, Info(next_entry, Querying(rid, key)), 0);
-  //     r := easy_transform_step(r, r', step);
+      glinear var rmutex;
+      ghost var left := oneRowResource(slot_idx' as nat, Info(next_entry, Querying(rid, key)), 0);
+      ghost var right := oneRowResource(slot_idx as nat, Info(entry, Free), 0);
+      r, rmutex := SSM.split(r, left, right);
+      v.row_mutexes[slot_idx].release(Row(entry, rmutex), handle);
 
-  //     glinear var rmutex;
-  //     ghost var left := oneRowResource(slot_idx' as nat, Info(next_entry, Querying(rid, key)), 0);
-  //     ghost var right := oneRowResource(slot_idx as nat, Info(entry, Free), 0);
-  //     r, rmutex := SSM.split(r, left, right);
-  //     v.row_mutexes[slot_idx].release(Row(entry, rmutex), handle);
-
-  //     slot_idx := slot_idx';
-  //     entry := next_entry;
-  //     handle := next_handle;
-  //   }
+      slot_idx := slot_idx';
+      entry := next_entry;
+      handle := next_handle;
+    }
     
-  //   // assert step.QueryNotFoundStep? || step.QueryDoneStep?;
-  //   r' := SSM.Variables(oneRowTable(slot_idx as nat, Info(entry, Free)), 0, multiset{}, multiset{Stub(rid, output)}); 
-  //   r := easy_transform_step(r, r', step);
+    // assert step.QueryNotFoundStep? || step.QueryDoneStep?;
+    r' := SSM.Variables(oneRowTable(slot_idx as nat, Info(entry, Free)), Count.Variables(0), multiset{}, multiset{Stub(rid, output)}); 
+    r := easy_transform_step(r, r', step);
 
-  //   glinear var rmutex;
-  //   r, rmutex := SSM.split(r, 
-  //     SSM.output_stub(rid, output), 
-  //     oneRowResource(slot_idx as nat, Info(entry, Free), 0));
-  //   v.row_mutexes[slot_idx].release(Row(entry, rmutex), handle);
+    glinear var rmutex;
+    r, rmutex := SSM.split(r, 
+      SSM.output_stub(rid, output), 
+      oneRowResource(slot_idx as nat, Info(entry, Free), 0));
+    v.row_mutexes[slot_idx].release(Row(entry, rmutex), handle);
 
-  //   out_sv := r;
-  // }
+    out_sv := r;
+  }
 
-  // method acquireCapacity(v: Variables, thread_id: uint32)
-  // returns (linear cap: AllocatorBin, glinear cap_handle: MutexHandle<AllocatorBin>, tid: uint32)
-  //   decreases *
-  //   requires Inv(v)
-  //   ensures cap.resource == unit().(insert_capacity := cap.count as nat)
-  //   ensures 0 < cap.count
-  //   ensures tid < CAP.BinCountImpl()
-  //   ensures cap_handle.m == v.allocator[tid]
-  // {
-  //   // thread_id is a hint for the bin we're supposed to use. 
-  //   // tid is the actual place we found the capacity (in case we had to steal it from someone else) 
-  //   tid := if thread_id >= CAP.BinCountImpl() then 0 else thread_id;
-  //   cap, cap_handle := v.allocator[tid].acquire();
+  method acquireCapacity(v: Variables, thread_id: uint32)
+  returns (linear cap: AllocatorBin, glinear cap_handle: MutexHandle<AllocatorBin>, tid: uint32)
+    decreases *
+    requires Inv(v)
+    ensures CAP.BinInv(cap)
+    ensures 0 < cap.count
+    ensures tid < CAP.NumberOfBinsImpl()
+    ensures cap_handle.m == v.allocator[tid]
+  {
+    // thread_id is a hint for the bin we're supposed to use. 
+    // tid is the actual place we found the capacity (in case we had to steal it from someone else) 
+    tid := if thread_id >= CAP.NumberOfBinsImpl() then 0 else thread_id;
+    cap, cap_handle := v.allocator[tid].acquire();
 
-  //   while true
-  //     invariant tid < CAP.BinCountImpl()
-  //     invariant cap.resource == unit().(insert_capacity := cap.count as nat)
-  //     invariant cap_handle.m == v.allocator[tid]
-  //     decreases *
-  //   {
-  //     if 0 < cap.count {
-  //       break;
-  //     }
+    while true
+      invariant tid < CAP.NumberOfBinsImpl()
+      invariant CAP.BinInv(cap)
+      invariant cap_handle.m == v.allocator[tid]
+      decreases *
+    {
+      if 0 < cap.count {
+        break;
+      }
 
-  //     // assert exists s' :: TableQuantityInv(add(s, s'))
-  //     assert CAP.BinInv(cap);
-  //     v.allocator[tid].release(cap, cap_handle);
+      // assert exists s' :: TableQuantityInv(add(s, s'))
+      assert CAP.BinInv(cap);
+      v.allocator[tid].release(cap, cap_handle);
 
-  //     tid := tid + 1;
-  //     tid := if tid >= CAP.BinCountImpl() then 0 else tid;
+      tid := tid + 1;
+      tid := if tid >= CAP.NumberOfBinsImpl() then 0 else tid;
 
-  //     cap, cap_handle := v.allocator[tid].acquire();
-  //   }
-  // }
+      cap, cap_handle := v.allocator[tid].acquire();
+    }
+  }
 
   // method doInsert(v: Variables, input: Ifc.Input, rid: int, thread_id: uint32, glinear in_sv: SSM.Variables)
   // returns (output: Ifc.Output, glinear out_sv: SSM.Variables)
